

ROLL NO : MS

--	--	--	--	--

 NAME :

PHY303 MidSem I (Part A) Date : Sep 11, 2023 Inst: Abhishek Chaudhuri

- Time : 30 minutes, Max Marks : 10
- Attempt all questions. Please give your answers in the space provided.

1. Write a differential equation that a Green function $G(\mathbf{r}, \mathbf{r}')$ for Poisson's equation must satisfy, for Dirichlet boundary conditions. Include a statement of the boundary conditions. [2]

$$\nabla^2 G(\mathbf{r}, \mathbf{r}') = -4\pi \delta^3(\mathbf{r} - \mathbf{r}') \text{ for } \mathbf{r}, \mathbf{r}' \text{ within } V \quad \text{--- (1)}$$

$$\text{B.C. } G(\mathbf{r}, \mathbf{r}') = 0 \text{ for } \mathbf{r} \text{ or } \mathbf{r}' \text{ on } S. \quad \text{--- (1)}$$

2. In an electrostatics problem with Neumann boundary conditions, what is the simplest allowable boundary condition on the the Green's function $G(\mathbf{r}, \mathbf{r}')$? Hint: The result must be consistent with the differential equation that G satisfies. [3]

$$\nabla^2 G(\mathbf{r}, \mathbf{r}') = -4\pi \delta^3(\mathbf{r} - \mathbf{r}') \text{ for } \mathbf{r}, \mathbf{r}' \text{ within } V$$

Integrating over volume V ,

$$\int_V \nabla^2 G(\mathbf{r}, \mathbf{r}') d^3 r' = -4\pi \int_V \delta^3(\mathbf{r} - \mathbf{r}') d^3 r' = -4\pi \quad \text{--- (1)}$$

$$\Rightarrow \int_V \vec{\nabla}' \cdot (\vec{\nabla}' G) d^3 r' = \oint_S \vec{\nabla}' G \cdot \hat{n}' da' \quad \text{Divergence Theorem.}$$

$$\therefore \oint_S \vec{\nabla}' G \cdot \hat{n}' da' = -4\pi$$

$$\Rightarrow \oint_S \frac{\partial G}{\partial n'} da' = -4\pi. \quad \text{--- (1)}$$

Choose, $\frac{\partial G}{\partial n'} = \text{const.} = A$ (say). Neumann B.C.

$$\therefore A \oint_S da' = -4\pi \Rightarrow A = -\frac{4\pi}{S}. \quad \text{--- (1)}$$

where S is total surface area of the system boundary.

3. Use delta-function to express the charge density $\rho(\mathbf{r})$ for the following charge distribution, in the indicated coordinate system: In spherical coordinates, a charge Q uniformly distributed over a spherical shell of radius R .

By symmetry, $\rho(\mathbf{r}) = \rho(r) = Q \delta(r - R) \cdot A$ — (1)
where A is some constant.

$$\text{Now, } Q = \int \rho(r, \theta, \phi) r^2 \sin \theta dr d\theta d\phi = 4\pi \int r^2 \rho(r) dr \\ = 4\pi Q A \int r^2 \delta(r - R) dr = 4\pi Q A R^2.$$

$$\therefore A = \frac{1}{4\pi R^2} \quad \therefore \rho(\mathbf{r}) = \frac{Q}{4\pi R^2} \delta(r - R). \text{ — (1)}$$

4. The continuity equation follows from charge conservation and is given as $\partial \rho / \partial t + \nabla \cdot \mathbf{J} = 0$. If the charge density is expressed as $\rho(\mathbf{r}, t) = \sum_k q_k \delta(\mathbf{r} - \mathbf{r}_k(t))$, find the expression for the current density $\mathbf{J}(\mathbf{r}, t)$? [3]

$$\rho = \sum_k q_k \delta(\mathbf{r} - \mathbf{r}_k(t)) \quad \therefore \frac{\partial \rho}{\partial t} = \sum_k q_k \frac{\partial}{\partial t} \delta(\mathbf{r} - \mathbf{r}_k(t)) \text{ — (1)} \\ \frac{\partial}{\partial t} \delta^3(\mathbf{r} - \mathbf{r}_k(t)) = \frac{\partial}{\partial t} [\delta(x - x_k(t)) \delta(y - y_k(t)) \delta(z - z_k(t))] \\ = \delta(y - y_k(t)) \delta(z - z_k(t)) \frac{\partial}{\partial t} \delta(x - x_k(t)) \\ + \dots \\ = -\delta(y - y_k(t)) \delta(z - z_k(t)) \frac{\partial}{\partial (x - x_k(t))} \delta(x - x_k(t)) \cdot \frac{\partial x_k}{\partial t} \\ \dots \\ = -\frac{\partial}{\partial (x - x_k)} [\delta(x - x_k(t)) \delta(y - y_k(t)) \delta(z - z_k(t))] \cdot \frac{\partial x_k}{\partial t} \\ - \frac{\partial}{\partial (y - y_k)} [\delta(x - x_k(t)) \delta(y - y_k(t)) \delta(z - z_k(t))] \cdot \frac{\partial y_k}{\partial t} \\ - \frac{\partial}{\partial (z - z_k)} [\delta(x - x_k(t)) \delta(y - y_k(t)) \delta(z - z_k(t))] \cdot \frac{\partial z_k}{\partial t} \\ = -\vec{v}_k \cdot \vec{\nabla} \delta^3(\mathbf{r} - \mathbf{r}_k(t)). \text{ — (1)} \text{ — (1)}$$

$$\therefore \frac{\partial \rho}{\partial t} = - \sum_k q_k \vec{v}_k \cdot \vec{\nabla} \delta^3(\mathbf{r} - \mathbf{r}_k(t))$$

$$= - \vec{\nabla} \cdot \left[\sum_k q_k \vec{v}_k \delta^3(\mathbf{r} - \mathbf{r}_k(t)) \right]$$

$$\therefore \vec{J} = \sum_k q_k \vec{v}_k \delta^3(\mathbf{r} - \mathbf{r}_k(t)). \text{ — (1)}$$

$$1. \quad \Phi(x, y) = (Ae^{kx} + Be^{-kx})(C \sin ky + D \cos ky).$$

B.C. : (i) $\Phi = 0$ when $y = 0$ (1)
 (ii) $\Phi = 0$ when $y = a$ (1)
 (iii) $\Phi = \Phi_0$ when $x = b$ (1)
 (iv) $\Phi = \Phi_0$ when $x = -b$ (1)

Since the region does not extend to $x \rightarrow \infty$, e^{kx} is fine. However Φ is symmetric w.r.t x .

$$\therefore \Phi(-x, y) = \Phi(x, y) \Rightarrow Ae^{-kx} + Be^{kx} = Ae^{kx} + Be^{-kx}$$

$$\Rightarrow (A - B)(e^{-kx} - e^{kx}) = 0$$

$$\therefore A = B. \quad (1)$$

$$\therefore \Phi(x, y) = A(e^{kx} + e^{-kx})(C \sin ky + D \cos ky)$$

$$= 2A \cosh kx (C' \sin ky + D' \cos ky).$$

where, $C' = 2AC$, $D' = 2AD$.

$$B.C.(i) \Rightarrow 0 = D' \cosh kx \Rightarrow D' = 0.$$

$$B.C.(ii) \Rightarrow 0 = C' \cosh kx \sin ka \Rightarrow \sin ka = 0.$$

$$\Rightarrow k = \frac{n\pi}{a}, \quad n = 1, 2, \dots \quad (1)$$

$$\therefore \Phi(x, y) = C' \cosh\left(\frac{n\pi x}{a}\right) \sin\left(\frac{n\pi y}{a}\right).$$

General solⁿ: $\Phi(x, y) = \sum_{n=1}^{\infty} C_n' \cosh\left(\frac{n\pi x}{a}\right) \sin\left(\frac{n\pi y}{a}\right)$

Pick C_n such that, B.C. (iii) is satisfied

$$\text{i.e., } \Phi(b, y) = \Phi_0 = \sum_{n=1}^{\infty} C_n' \cosh\left(\frac{n\pi b}{a}\right) \sin\left(\frac{n\pi y}{a}\right).$$

Multiplying both sides by $\sin\left(\frac{n'\pi y}{a}\right)$ and integrating from 0 to a,

$$\begin{aligned} \sum_{n=1}^{\infty} C_n \left[\int_0^a dy \sin\left(\frac{n\pi y}{a}\right) \sin\left(\frac{n'\pi y}{a}\right) \right] \cosh\left(\frac{n\pi b}{a}\right) &= \int_0^a dy \Phi_0 \sin\left(\frac{n'\pi y}{a}\right) \\ &= \Phi_0 \int_0^a \sin\left(\frac{n'\pi y}{a}\right) dy \\ &= -\Phi_0 \cdot \frac{a}{n'\pi} \left[\cos\left(\frac{n'\pi y}{a}\right) \right]_0^a \end{aligned}$$

$$\Rightarrow \frac{a}{2} \sum_{n=1}^{\infty} C_n \cosh\left(\frac{n\pi b}{a}\right) \delta_{n'n} = \frac{\Phi_0 a}{n'\pi} (1 - \cos n\pi)$$

$$\Rightarrow C_{n'} \cosh\left(\frac{n'\pi b}{a}\right) = \frac{2\Phi_0}{n'\pi} (1 - \cos n\pi) = \begin{cases} 0 & n' = \text{even} \\ \frac{4\Phi_0}{n'\pi} & n' = \text{odd} \end{cases}$$

① $\therefore \Phi(x, y) = \frac{4\Phi_0}{\pi} \sum_{n=1,3,5,\dots} \frac{1}{n} \frac{\cosh(n\pi x/a)}{\cosh(n\pi b/a)} \sin\left(\frac{n\pi y}{a}\right)$

2. Potential on the sphere is zero.

$$\text{Then, } \Phi(\vec{r}) = \frac{1}{4\pi\epsilon_0} \int \rho(\vec{r}') G_D(\vec{r}, \vec{r}') d^3r'$$

$$\rho(\vec{r}') = Q \delta(\vec{r}' + a\hat{k}) - Q \delta(\vec{r}' - a\hat{k})$$

$$\therefore \Phi(\vec{r}) = \frac{Q}{4\pi\epsilon_0} \int_V [\delta(\vec{r}' + a\hat{k}) - \delta(\vec{r}' - a\hat{k})] G_D(\vec{r}, \vec{r}') d^3r'$$

$$= \frac{Q}{4\pi\epsilon_0} [G_D(\vec{r}, -a\hat{k}) - G_D(\vec{r}, a\hat{k})] \quad (1)$$

$$\text{Now, } G_D(\vec{r}, \vec{r}') = \frac{1}{|\vec{r} - \vec{r}'|} - \frac{R/r'}{|\vec{r} - \frac{R^2}{r'^2} \vec{r}'|}$$

$$= \frac{1}{\sqrt{r^2 + r'^2 - 2rr'\cos\gamma}} - \frac{1}{\sqrt{\frac{r^2 r'^2}{R^2} + R^2 - 2rr'\cos\gamma}}$$

where γ is the angle between \vec{r} & \vec{r}' .

Hence, $\cos\gamma \equiv \cos\theta$.

$$\therefore G_D(\vec{r}, a\hat{k}) = \frac{1}{\sqrt{r^2 + a^2 - 2ar\cos\theta}} - \frac{1}{\sqrt{\frac{r^2 a^2}{R^2} + R^2 - 2ar\cos\theta}}$$

$$= \frac{1}{a} \frac{1}{\sqrt{1 + \frac{r^2}{a^2} - 2\frac{r}{a}\cos\theta}} - \frac{R}{ra} \frac{1}{\sqrt{1 + \frac{R^4}{a^2 r^2} - 2\frac{R}{ar}\cos\theta}} \quad (1)$$

Similarly,

$$G_D(\vec{r}, -a\hat{k}) = \frac{1}{a} \frac{1}{\sqrt{1 + \frac{r^2}{a^2} + 2\frac{r}{a}\cos\theta}} - \frac{R}{ra} \frac{1}{\sqrt{1 + \frac{R^4}{a^2 r^2} + 2\frac{R}{ar}\cos\theta}} \quad (1)$$

When $a \gg R$, i.e. the sources are at infinity,

$$G_D(\vec{r}, a\hat{k}) \approx \frac{1}{a} \left(1 + \frac{r}{a} \cos\theta - \frac{r^2}{2a^2} \right) - \frac{R}{ar} \left(1 + \frac{R^2}{ar} \cos\theta - \frac{R^4}{2a^2 r^2} \right)$$

$$\& C_D(\vec{r}, -R\hat{n}) \approx \frac{1}{a} \left(1 - \frac{r}{a} \cos\theta + \frac{r^2}{2a^2} \right) - \frac{R}{a^2} \left(1 - \frac{R}{a} \cos\theta - \frac{R^2}{2a^2} \right)$$

$$\therefore \Phi(\vec{r}) = \frac{Q}{4\pi\epsilon_0} \left[\frac{1}{a} \left(1 - \frac{r}{a} \cos\theta + \frac{r^2}{2a^2} \right) - \frac{R}{a^2} \left(1 - \frac{R}{a} \cos\theta - \frac{R^2}{2a^2} \right) - \frac{1}{a} \left(1 + \frac{r}{a} \cos\theta - \frac{r^2}{2a^2} \right) + \frac{R}{a^2} \left(1 + \frac{R}{a} \cos\theta - \frac{R^2}{2a^2} \right) \right]$$

①

$$= \frac{Q}{4\pi\epsilon_0} \left[\frac{2}{a} \left(\frac{r^2}{2a^2} - \frac{r}{a} \cos\theta \right) + \frac{2R}{a^2} \left(-\frac{R^2}{2a^2} + \frac{R^2}{a^2} \cos\theta \right) \right]$$

For large 'a', we can further approximate this:

$$\Phi(\vec{r}) \approx \frac{Q}{4\pi\epsilon_0} \left[-\frac{2}{a} \cdot \frac{r}{a} \cos\theta + \frac{2R}{a^2} \cdot \frac{R^2}{a^2} \cos\theta \right]$$

$$= -\left(\frac{2Q}{4\pi\epsilon_0 a} \right) r \cos\theta + \left(\frac{2Q}{4\pi\epsilon_0 a^2} \right) \cdot \frac{R^3}{a^2} \cos\theta.$$

①

The uniform field produced by the external charges kept far apart is, $E_0 = \frac{2Q}{4\pi\epsilon_0 a^2}$.

$$\therefore \Phi(\vec{r}) = -E_0 r \cos\theta + \frac{E_0 a^3}{r} \cos\theta.$$

potential due to
unif. field E_0

potential due to induced
surface charge

Surface charge density,

$$\begin{aligned} \sigma &= -\epsilon_0 \left. \frac{\partial \Phi}{\partial r} \right|_{r=R} = \epsilon_0 E_0 \left(1 + \frac{2R^3}{r^3} \right) \bigg|_{r=R} \cos\theta \\ &= \epsilon_0 E_0 \left(1 + \frac{2R^3}{R^3} \right) \cos\theta \\ &= 3\epsilon_0 E_0 \cos\theta. \end{aligned}$$